src/FlatSeqStmt.v
@@ -7,18 +7,20 @@ Require Import Monads.
 Require Export HigherValue.
 Require Import ListLemmas.
 
-Inductive insn :=
+Inductive stmt :=
+| Skip
+| Seq (s1 : stmt) (s2 : stmt)
 | Arg (dst : nat)
 | Self (dst : nat)
 | Deref (dst : nat) (e : nat) (off : nat)
 | Call (dst : nat) (f : nat) (a : nat)
 | MkConstr (dst : nat) (tag : nat) (args : list nat)
-| Switch (dst : nat) (cases : list (list insn))
+| Switch (dst : nat) (cases : list stmt)
 | MkClose (dst : nat) (f : function_name) (free : list nat)
 | Copy (dst : nat) (src : nat)
 .
 
-Definition env := list (list insn * nat).
+Definition env := list (stmt * nat).
 
 
 (* Continuation-based step relation *)
@@ -37,53 +39,52 @@ Definition local f l := lookup (locals f) l.
 
 
 Inductive cont :=
-| Kseq (code : list insn) (k : cont)
+| Kseq (code : stmt) (k : cont)
 | Kswitch (k : cont)
 | Kret (ret : nat) (dst : nat) (f : frame) (k : cont)
 | Kstop (ret : nat).
 
 Inductive state :=
-| Run (i : list insn) (f : frame) (k : cont)
+| Run (s : stmt) (f : frame) (k : cont)
 | Stop (v : value).
 
 Inductive sstep (E : env) : state -> state -> Prop :=
-| SSeq : forall i is f k,
-        is <> [] ->
-        sstep E (Run (i :: is) f k)
-                (Run [i] f (Kseq is k))
+| SSeq : forall s1 s2 f k,
+        sstep E (Run (Seq s1 s2) f k)
+                (Run s1 f (Kseq s2 k))
 
 | SArg : forall dst f k,
-        sstep E (Run [Arg dst] f k)
-                (Run [] (set f dst (arg f)) k)
+        sstep E (Run (Arg dst) f k)
+                (Run Skip (set f dst (arg f)) k)
 | SSelf : forall dst f k,
-        sstep E (Run [Self dst] f k)
-                (Run [] (set f dst (self f)) k)
+        sstep E (Run (Self dst) f k)
+                (Run Skip (set f dst (self f)) k)
 
 | SDerefinateConstr : forall dst e off f k  tag args v,
         local f e = Some (Constr tag args) ->
         nth_error args off = Some v ->
-        sstep E (Run [Deref dst e off] f k)
-                (Run [] (set f dst v) k)
+        sstep E (Run (Deref dst e off ) f k)
+                (Run Skip (set f dst v) k)
 | SDerefinateClose : forall dst e off f k  fname free v,
         local f e = Some (Close fname free) ->
         nth_error free off = Some v ->
-        sstep E (Run [Deref dst e off] f k)
-                (Run [] (set f dst v) k)
+        sstep E (Run (Deref dst e off ) f k)
+                (Run Skip (set f dst v) k)
 
 | SConstrDone : forall dst tag args f k vs,
         Forall2 (fun l v => local f l = Some v) args vs ->
-        sstep E (Run [MkConstr dst tag args] f k)
-                (Run [] (set f dst (Constr tag vs)) k)
+        sstep E (Run (MkConstr dst tag args ) f k)
+                (Run Skip (set f dst (Constr tag vs)) k)
 | SCloseDone : forall dst fname free f k vs,
         Forall2 (fun l v => local f l = Some v) free vs ->
-        sstep E (Run [MkClose dst fname free] f k)
-                (Run [] (set f dst (Close fname vs)) k)
+        sstep E (Run (MkClose dst fname free ) f k)
+                (Run Skip (set f dst (Close fname vs)) k)
 
 | SMakeCall : forall dst fl a f k  fname free arg body ret,
         local f fl = Some (Close fname free) ->
         local f a = Some arg ->
         nth_error E fname = Some (body, ret) ->
-        sstep E (Run [Call dst fl a] f k)
+        sstep E (Run (Call dst fl a ) f k)
                 (Run body (Frame arg (Close fname free) [])
                     (Kret ret dst f k))
 
@@ -91,27 +92,27 @@ Inductive sstep (E : env) : state -> state -> Prop :=
 | SSwitchinate : forall dst cases f k  tag args case,
         arg f = Constr tag args ->
         nth_error cases tag = Some case ->
-        sstep E (Run [Switch dst cases] f k)
+        sstep E (Run (Switch dst cases) f k)
                 (Run case f (Kswitch k))
 
 | SCopy : forall dst src f k v,
         local f src = Some v ->
-        sstep E (Run [Copy dst src] f k)
-                (Run [] (set f dst v) k)
+        sstep E (Run (Copy dst src ) f k)
+                (Run Skip (set f dst v) k)
 
-| SContSeq : forall code f k,
-        sstep E (Run [] f (Kseq code k))
-                (Run code f k)
+| SContSeq : forall f s k,
+        sstep E (Run Skip f (Kseq s k))
+                (Run s f k)
 | SContSwitch : forall f k,
-        sstep E (Run [] f (Kswitch k))
-                (Run [] f k)
+        sstep E (Run Skip f (Kswitch k))
+                (Run Skip f k)
 | SContRet : forall f ret dst f' k v,
         local f ret = Some v ->
-        sstep E (Run [] f (Kret ret dst f' k))
-                (Run [] (set f' dst v) k)
+        sstep E (Run Skip f (Kret ret dst f' k))
+                (Run Skip (set f' dst v) k)
 | SContStop : forall ret f v,
         local f ret = Some v ->
-        sstep E (Run [] f (Kstop ret))
+        sstep E (Run Skip f (Kstop ret))
                 (Stop v)
 .
 
@@ -137,94 +138,53 @@ Inductive splus (E : env) : state -> state -> Prop :=
  * Mutual recursion/induction schemes for expr
  *)
 
-Definition insn_rect_mut
-        (P : insn -> Type)
-        (Pl : list insn -> Type)
-        (Pll : list (list insn) -> Type)
+Definition stmt_rect_mut
+        (P : stmt -> Type)
+        (Pl : list stmt -> Type)
+    (HSkip :    P Skip)
+    (HSeq :     forall s1 s2, P s1 -> P s2 -> P (Seq s1 s2))
     (HArg :     forall dst, P (Arg dst))
     (HSelf :    forall dst, P (Self dst))
     (HDeref :   forall dst e off, P (Deref dst e off))
     (HCall :    forall dst f a, P (Call dst f a))
     (HConstr :  forall dst tag args, P (MkConstr dst tag args))
-    (HSwitch :  forall dst cases, Pll cases -> P (Switch dst cases))
+    (HSwitch :  forall dst cases, Pl cases -> P (Switch dst cases))
     (HClose :   forall dst fname free, P (MkClose dst fname free))
     (HCopy :    forall dst src, P (Copy dst src))
     (Hnil :     Pl [])
     (Hcons :    forall i is, P i -> Pl is -> Pl (i :: is))
-    (Hnil2 :    Pll [])
-    (Hcons2 :   forall is iss, Pl is -> Pll iss -> Pll (is :: iss))
-    (i : insn) : P i :=
+    (i : stmt) : P i :=
     let fix go i :=
         let fix go_list is :=
             match is as is_ return Pl is_ with
             | [] => Hnil
             | i :: is => Hcons i is (go i) (go_list is)
             end in
-        let fix go_list_list iss :=
-            match iss as iss_ return Pll iss_ with
-            | [] => Hnil2
-            | is :: iss => Hcons2 is iss (go_list is) (go_list_list iss)
-            end in
         match i as i_ return P i_ with
+        | Skip => HSkip
+        | Seq s1 s2 => HSeq s1 s2 (go s1) (go s2)
         | Arg dst => HArg dst
         | Self dst => HSelf dst
         | Deref dst e off => HDeref dst e off
         | Call dst f a => HCall dst f a
         | MkConstr dst tag args => HConstr dst tag args
-        | Switch dst cases => HSwitch dst cases (go_list_list cases)
+        | Switch dst cases => HSwitch dst cases (go_list cases)
         | MkClose dst fname free => HClose dst fname free
         | Copy dst src => HCopy dst src
         end in go i.
 
 (* Useful wrapper for `expr_rect_mut with (Pl := Forall P)` *)
-Definition insn_ind' (P : insn -> Prop)
+Definition stmt_ind' (P : stmt -> Prop)
+    (HSkip :    P Skip)
+    (HSeq :     forall s1 s2, P s1 -> P s2 -> P (Seq s1 s2))
     (HArg :     forall dst, P (Arg dst))
     (HSelf :    forall dst, P (Self dst))
     (HDeref :   forall dst e off, P (Deref dst e off))
     (HCall :    forall dst f a, P (Call dst f a))
     (HConstr :  forall dst tag args, P (MkConstr dst tag args))
-    (HSwitch :  forall dst cases, Forall (Forall P) cases -> P (Switch dst cases))
+    (HSwitch :  forall dst cases, Forall P cases -> P (Switch dst cases))
     (HClose :   forall dst fname free, P (MkClose dst fname free))
     (HCopy :    forall dst src, P (Copy dst src))
-    (i : insn) : P i :=
-    ltac:(refine (@insn_rect_mut P (Forall P) (Forall (Forall P))
-        HArg HSelf HDeref HCall HConstr HSwitch HClose HCopy _ _ _ _ i); eauto).
-
-Definition insn_list_rect_mut
-        (P : insn -> Type)
-        (Pl : list insn -> Type)
-        (Pll : list (list insn) -> Type)
-    (HArg :     forall dst, P (Arg dst))
-    (HSelf :    forall dst, P (Self dst))
-    (HDeref :   forall dst e off, P (Deref dst e off))
-    (HCall :    forall dst f a, P (Call dst f a))
-    (HConstr :  forall dst tag args, P (MkConstr dst tag args))
-    (HSwitch :  forall dst cases, Pll cases -> P (Switch dst cases))
-    (HClose :   forall dst fname free, P (MkClose dst fname free))
-    (HCopy :    forall dst src, P (Copy dst src))
-    (Hnil :     Pl [])
-    (Hcons :    forall i is, P i -> Pl is -> Pl (i :: is))
-    (Hnil2 :    Pll [])
-    (Hcons2 :   forall is iss, Pl is -> Pll iss -> Pll (is :: iss))
-    (is : list insn) : Pl is :=
-    let go := insn_rect_mut P Pl Pll
-            HArg HSelf HDeref HCall HConstr HSwitch HClose HCopy Hnil Hcons Hnil2 Hcons2 in
-    let fix go_list is :=
-        match is as is_ return Pl is_ with
-        | [] => Hnil
-        | i :: is => Hcons i is (go i) (go_list is)
-        end in go_list is.
-
-
-
-Definition dest e :=
-    match e with
-    | Arg dst => dst
-    | Self dst => dst
-    | Deref dst _ _ => dst
-    | Call dst _ _ => dst
-    | MkConstr dst _ _ => dst
-    | Switch dst _ => dst
-    | MkClose dst _ _ => dst
-    | Copy dst _ => dst
-    end.
+    (i : stmt) : P i :=
+    ltac:(refine (@stmt_rect_mut P (Forall P)
+        HSkip HSeq HArg HSelf HDeref HCall HConstr HSwitch HClose HCopy _ _ i); eauto).
